Batteries/Data/Float/Lemmas.lean
@@ -1,0 +1,303 @@
+/-
+Copyright (c) 2026 Robin Arnez. All rights reserved.
+Released under Apache 2.0 license as described in the file LICENSE.
+Authors: Robin Arnez
+-/
+module
+public import Batteries.Data.Float.Basic
+import all Init.Data.OfScientific
+
+@[expose] public section
+
+namespace Float.Model.UnpackedFloat
+
+/-- Returns true if the bits represent an NaN value -/
+def isNaNBits {spec : Format} (b : BitVec spec.numBits) : Bool :=
+  unpackExponent b = -1#_ ∧ unpackMantissa b ≠ 0#_
+
+namespace Sign
+
+@[simp]
+theorem ofBitVec_toBitVec (s : Sign) :
+    Sign.ofBitVec s.toBitVec = s := by
+  cases s <;> rfl
+
+@[simp]
+theorem toBitVec_ofBitVec (b : BitVec 1) :
+    (Sign.ofBitVec b).toBitVec = b := by
+  decide +revert
+
+protected theorem forall_iff {p : Sign → Prop} :
+    (∀ s : Sign, p s) ↔ p .positive ∧ p .negative := by
+  constructor
+  · intro h; simp [h]
+  · rintro ⟨h, h'⟩ (_ | _) <;> assumption
+
+instance {p : Sign → Prop} [∀ s, Decidable (p s)] : Decidable (∀ s : Sign, p s) :=
+  decidable_of_decidable_of_iff Sign.forall_iff.symm
+
+deriving instance DecidableEq for Sign
+
+instance : Std.LawfulEqOrd Sign where
+  compare_self := by decide
+  eq_of_compare := by decide
+
+instance : Std.TransOrd Sign where
+  eq_swap := by decide
+  isLE_trans := by decide
+
+end Sign
+
+theorem unpackMantissa_def {spec : Format} (b : BitVec spec.numBits) :
+    unpackMantissa b = b.extractLsb' 0 spec.mantissaBitsWithoutImplicit := by
+  ext; simp [unpackMantissa, BitVec.extractLsb]
+
+theorem unpackExponent_def {spec : Format} (b : BitVec spec.numBits) :
+    unpackExponent b = b.extractLsb' spec.mantissaBitsWithoutImplicit spec.exponentBits := by
+  ext; simp [unpackExponent, BitVec.extractLsb]
+
+theorem unpackSign_def {spec : Format} (b : BitVec spec.numBits) :
+    unpackSign b = b.extractLsb' (spec.mantissaBitsWithoutImplicit + spec.exponentBits) 1 := by
+  ext; simp [unpackSign, BitVec.extractLsb]
+
+@[simp]
+theorem unpackSign_packComponents {spec : Format} (s e m) :
+    unpackSign (packComponents spec s e m) = s.toBitVec := by
+  ext i (_ | ⟨⟨⟩⟩)
+  simp +arith [unpackSign_def, packComponents, BitVec.getElem_append]
+
+theorem packComponents_unpackSign_unpackExponent_unpackMantissa
+    {spec : Format} (b : BitVec spec.numBits) :
+    packComponents spec (Sign.ofBitVec (unpackSign b)) (unpackExponent b) (unpackMantissa b) = b := by
+  simp [packComponents]
+  rw [unpackSign_def, unpackExponent_def, unpackMantissa_def]
+  rw [BitVec.extractLsb'_append_extractLsb'_eq_extractLsb',
+    BitVec.extractLsb'_append_extractLsb'_eq_extractLsb']
+  · exact BitVec.extractLsb'_eq_self
+  · simp
+  · simp
+
+theorem pack_unpack {spec : Format} (b : BitVec spec.numBits)
+    (hspec : 2 ≤ spec.exponentBits := by decide) :
+    (unpack spec b).pack spec = if isNaNBits b then packedNaN spec else b := by
+  conv => rhs; rw [← packComponents_unpackSign_unpackExponent_unpackMantissa b]
+  unfold isNaNBits
+  fun_cases unpack with
+  | case1 mvec evec svec s hevec hmvec =>
+    -- infinity
+    simp +zetaDelta [pack, packedInfinity, hmvec, hevec]
+  | case2 mvec evec hevec hmvec =>
+    -- nan
+    simp +zetaDelta [pack, packedNaN, hevec, hmvec]
+  | case3 mvec evec svec s _ hevec hmvec =>
+    -- zero
+    simp +zetaDelta [pack, packedZero, hevec, hmvec]
+  | case4 mvec evec e svec s _ hevec hmvec =>
+    -- subnormal
+    simp only [hevec, unpackExponent_packComponents, BitVec.zero_eq_neg_one_iff,
+      Nat.ne_of_gt spec.he, unpackMantissa_packComponents, ne_eq, false_and, decide_false,
+      Bool.false_eq_true, ↓reduceIte, evec]
+    unfold pack
+    extract_lets mantbits biasedexp
+    simp only [BitVec.ofNat_toNat, BitVec.setWidth_eq, mvec]
+    rw [if_neg, if_neg]
+    · rw [Format.mantissaBits, Nat.add_comm, Nat.add_left_cancel_iff]
+      apply Nat.ne_of_lt
+      have := mt BitVec.toNat_inj.mp hmvec
+      simp only [BitVec.toNat_ofNat, Nat.zero_mod] at this
+      simp only [ne_eq, this, not_false_eq_true, Nat.log2_lt, gt_iff_lt, mantbits]
+      exact BitVec.isLt _
+    · simp +arith [biasedexp, e, hevec]
+      have := Nat.pow_le_pow_right (n := 2) (by decide) hspec
+      lia
+  | case5 mvec evec e svec s hevec hevec' =>
+    -- normal
+    simp only [unpackExponent_packComponents, hevec, unpackMantissa_packComponents, ne_eq,
+      false_and, decide_false, Bool.false_eq_true, ↓reduceIte, evec]
+    unfold pack
+    extract_lets mantbits biasedexp
+    rw [if_neg, if_pos]
+    · congr
+      · simp +arith [biasedexp, e, evec]
+      · rw [BitVec.ofNat_toNat, BitVec.setWidth_append]
+        simp [mvec]
+    · subst mantbits
+      have := Nat.two_pow_add_eq_or_of_lt mvec.isLt (a := 1)
+      rw [Nat.mul_one] at this
+      simp only [BitVec.toNat_append, BitVec.toNat_ofNat, Nat.pow_one, Nat.mod_succ,
+        Format.mantissaBits, Nat.add_comm 1, Nat.add_right_cancel_iff,
+        Nat.one_shiftLeft, ← this]
+      rw [Nat.log2_eq_iff (by simp)]
+      simp [Nat.two_pow_succ, mvec.isLt]
+    · simp +arith [biasedexp, e]
+      simp only [BitVec.neg_one_eq_allOnes, ← BitVec.lt_allOnes_iff, BitVec.lt_def,
+        BitVec.toNat_allOnes] at hevec
+      lia
+
+theorem pack_unpack_of_valid {spec : Format} {b : BitVec spec.numBits}
+    (hvalid : spec.Valid b) (hspec : 2 ≤ spec.exponentBits := by decide) :
+    (unpack spec b).pack spec = b := by
+  rw [pack_unpack b hspec]
+  simp +contextual [isNaNBits, ← hvalid.eq_packedNaN]
+
+theorem unpack_inj_of_valid {spec : Format} {b b' : BitVec spec.numBits}
+    (hb : spec.Valid b) (hb' : spec.Valid b') (hspec : 2 ≤ spec.exponentBits := by decide) :
+    unpack spec b = unpack spec b' ↔ b = b' := by
+  constructor
+  · intro h
+    replace h := congrArg (pack spec) h
+    rwa [pack_unpack_of_valid hb hspec, pack_unpack_of_valid hb' hspec] at h
+  · rintro rfl; rfl
+
+theorem isNaNBits_packedNaN {spec : Format} : isNaNBits (packedNaN spec) := by
+  simp only [isNaNBits, packedNaN, unpackExponent_packComponents, unpackMantissa_packComponents,
+    ne_eq, true_and, decide_not, Bool.not_eq_eq_eq_not, Bool.not_true, decide_eq_false_iff_not]
+  intro h
+  replace h := congrArg (·.getLsbD (spec.mantissaBitsWithoutImplicit - 1)) h
+  simp [Nat.sub_one_lt (Nat.ne_of_gt spec.hm)] at h
+
+@[simp]
+theorem unpack_packedNaN {spec : Format} : unpack spec (packedNaN spec) = notANumber := by
+  have := @isNaNBits_packedNaN spec
+  simp only [isNaNBits, decide_eq_true_eq] at this
+  simp [unpack, this]
+
+@[simp]
+theorem unpack_packedZero {spec : Format} {sign : Sign} : unpack spec (packedZero spec sign) = .zero sign := by
+  simp [unpack, packedZero, Nat.ne_of_gt spec.he]
+
+@[simp]
+theorem isNaN_iff : isNaN x ↔ x = notANumber := by
+  cases x <;> simp [isNaN]
+
+theorem unpack_eq_notANumber_iff_of_valid {spec : Format} {b : BitVec spec.numBits}
+    (hvalid : spec.Valid b) (hspec : 2 ≤ spec.exponentBits := by decide) :
+    unpack spec b = notANumber ↔ b = packedNaN spec := by
+  rw [← @unpack_packedNaN spec, unpack_inj_of_valid hvalid ⟨fun _ _ => rfl⟩ hspec]
+
+theorem unpack_eq_zero_iff_of_valid {spec : Format} {sign : Sign} {b : BitVec spec.numBits}
+    (hvalid : spec.Valid b) (hspec : 2 ≤ spec.exponentBits := by decide) :
+    unpack spec b = zero sign ↔ b = packedZero spec sign := by
+  rw [← @unpack_packedZero spec, unpack_inj_of_valid hvalid ⟨by simp [packedZero]⟩ hspec]
+
+theorem isNaN_unpack_iff_of_valid {spec : Format} {b : BitVec spec.numBits}
+    (hvalid : spec.Valid b) (hspec : 2 ≤ spec.exponentBits := by decide) :
+    (unpack spec b).isNaN ↔ b = packedNaN spec := by
+  rw [isNaN_iff, unpack_eq_notANumber_iff_of_valid hvalid hspec]
+
+theorem beq_iff_ne_notANumber_and_eq (a b : UnpackedFloat) :
+    a.beq b ↔ a ≠ notANumber ∧ b ≠ notANumber ∧
+      (a = b ∨ (a = .zero .positive ∧ b = .zero .negative) ∨
+        (a = .zero .negative ∧ b = .zero .positive)) := by
+  simp only [UnpackedFloat.beq, beq_iff_eq, ne_eq]
+  fun_cases UnpackedFloat.compare a b <;> simp_all [eq_comm (α := UnpackedFloat), and_comm]
+  decide +revert -- inf/inf
+
+theorem unpack_beq_unpack_iff {spec : Format} {b b' : BitVec spec.numBits}
+    (hb : spec.Valid b) (hb' : spec.Valid b') (hspec : 2 ≤ spec.exponentBits := by decide) :
+    (unpack spec b).beq (unpack spec b') ↔ b ≠ packedNaN spec ∧ b' ≠ packedNaN spec ∧
+        (b = b' ∨ (b = packedZero spec .positive ∧ b' = packedZero spec .negative) ∨
+          (b = packedZero spec .negative ∧ b' = packedZero spec .positive)) := by
+  rw [beq_iff_ne_notANumber_and_eq]
+  simp [unpack_eq_notANumber_iff_of_valid, unpack_eq_zero_iff_of_valid, unpack_inj_of_valid, *]
+
+end Float.Model.UnpackedFloat
+
+theorem Float.toBits_inj {f f' : Float} : f.toBits = f'.toBits ↔ f = f' := by
+  rcases f with ⟨⟨⟩⟩; rcases f' with ⟨⟨⟩⟩; simp [toBits]
+
+theorem Float32.toBits_inj {f f' : Float32} : f.toBits = f'.toBits ↔ f = f' := by
+  rcases f with ⟨⟨⟩⟩; rcases f' with ⟨⟨⟩⟩; simp [toBits]
+
+@[simp]
+theorem Float.ofBits_toBits (f : Float) : ofBits f.toBits = f :=
+  toBits_inj.mp <| UInt64.toBitVec_inj.mp <|
+    Float.Model.UnpackedFloat.pack_unpack_of_valid f.toModel.valid
+
+@[simp]
+theorem Float32.ofBits_toBits (f : Float32) : ofBits f.toBits = f :=
+  toBits_inj.mp <| UInt32.toBitVec_inj.mp <|
+    Float.Model.UnpackedFloat.pack_unpack_of_valid f.toModel.valid
+
+@[simp]
+theorem Float.isNaN_eq_decide_eq_nan {f : Float} : isNaN f = decide (f = nan) := by
+  rw [Bool.eq_iff_iff, decide_eq_true_eq, ← toBits_inj, ← UInt64.toBitVec_inj]
+  exact Float.Model.UnpackedFloat.isNaN_unpack_iff_of_valid f.toModel.valid
+
+@[simp]
+theorem Float32.isNaN_eq_decide_eq_nan {f : Float32} : isNaN f = decide (f = nan) := by
+  rw [Bool.eq_iff_iff, decide_eq_true_eq, ← toBits_inj, ← UInt32.toBitVec_inj]
+  exact Float.Model.UnpackedFloat.isNaN_unpack_iff_of_valid f.toModel.valid
+
+theorem Float.beq_iff_ne_nan_and_eq {f f' : Float} :
+    f == f' ↔ f ≠ nan ∧ f' ≠ nan ∧ (f = f' ∨ (f = 0 ∧ f' = -0) ∨ (f = -0 ∧ f' = 0)) := by
+  simp only [ne_eq, ← toBits_inj, ← UInt64.toBitVec_inj]
+  exact Float.Model.UnpackedFloat.unpack_beq_unpack_iff f.toModel.valid f'.toModel.valid
+
+theorem Float32.beq_iff_ne_nan_and_eq {f f' : Float32} :
+    f == f' ↔ f ≠ nan ∧ f' ≠ nan ∧ (f = f' ∨ (f = 0 ∧ f' = -0) ∨ (f = -0 ∧ f' = 0)) := by
+  simp only [ne_eq, ← toBits_inj, ← UInt32.toBitVec_inj]
+  exact Float.Model.UnpackedFloat.unpack_beq_unpack_iff f.toModel.valid f'.toModel.valid
+
+@[simp]
+theorem Float.nan_beq_eq_false (f : Float) : (nan == f) = false := by
+  simp [← Bool.not_eq_true, beq_iff_ne_nan_and_eq]
+
+@[simp]
+theorem Float32.nan_beq_eq_false (f : Float32) : (nan == f) = false := by
+  simp [← Bool.not_eq_true, beq_iff_ne_nan_and_eq]
+
+@[simp]
+theorem Float.beq_nan_eq_false (f : Float) : (f == nan) = false := by
+  simp [← Bool.not_eq_true, beq_iff_ne_nan_and_eq]
+
+@[simp]
+theorem Float32.beq_nan_eq_false (f : Float32) : (f == nan) = false := by
+  simp [← Bool.not_eq_true, beq_iff_ne_nan_and_eq]
+
+@[simp]
+theorem Float.beq_self_iff {f : Float} : f == f ↔ f ≠ nan := by
+  grind [beq_iff_ne_nan_and_eq]
+
+@[simp]
+theorem Float32.beq_self_iff {f : Float32} : f == f ↔ f ≠ nan := by
+  grind [beq_iff_ne_nan_and_eq]
+
+@[simp]
+theorem Float.beq_self_eq_false_iff {f : Float} : (f == f) = false ↔ f = nan := by
+  grind [beq_self_iff]
+
+@[simp]
+theorem Float32.beq_self_eq_false_iff {f : Float32} : (f == f) = false ↔ f = nan := by
+  grind [beq_self_iff]
+
+/--
+This theorem is true in general but most other types have `LawfulBEq` where
+`bne_self_eq_false` or `bne_iff_ne` apply.
+-/
+@[simp] theorem Float.bne_eq {f : Float} : (f != f) = (!f == f) := (rfl)
+
+/--
+This theorem is true in general but most other types have `LawfulBEq` where
+`bne_self_eq_false` or `bne_iff_ne` apply.
+-/
+@[simp] theorem Float32.bne_eq {f : Float32} : (f != f) = (!f == f) := (rfl)
+
+instance : PartialEquivBEq Float where
+  symm := by grind [Float.beq_iff_ne_nan_and_eq]
+  trans := by grind [Float.beq_iff_ne_nan_and_eq]
+
+instance : PartialEquivBEq Float32 where
+  symm := by grind [Float32.beq_iff_ne_nan_and_eq]
+  trans := by grind [Float32.beq_iff_ne_nan_and_eq]
+
+-- but!
+example : ¬ EquivBEq Float := by
+  intro h
+  have : Float.nan == Float.nan := BEq.rfl
+  contradiction
+
+example : ¬ EquivBEq Float32 := by
+  intro h
+  have : Float32.nan == Float32.nan := BEq.rfl
+  contradiction
